

# 1 Some Exercises in Real Analysis

## 1.1 (Sequences)

1. Prove the following sequential limits:

$$a) \lim_{n \rightarrow \infty} \frac{\sin(n)}{n} = 0, \quad b) \lim_{n \rightarrow \infty} \frac{n!}{n^n} = 0, \quad c) \lim_{n \rightarrow \infty} \frac{(1 + 2 + \cdots + n)^2}{n^4} = \frac{1}{4}.$$

Try proving in multiple ways ( $N - \varepsilon$ , squeeze theorem, etc).

(Hint (for b)): how many times does  $n$  appear in " $n!$ "? How about " $n^n$ "?)

2. The following sequences are defined recursively. Prove that each converges, and find the limiting value in each case.

$$a) \quad x_1 := \sqrt{2}, x_{n+1} := \sqrt{2 + x_n} \text{ for } n \geq 1$$

$$b) \quad x_1 = 2, x_{n+1} := \frac{1}{2} \left( x_n + \frac{2}{x_n} \right)$$

$$c) \quad x_1 := 1, x_2 := 2, x_{n+1} := \frac{1}{2}(x_n + x_{n-1})$$

$$d) \quad x_1 = 1, x_{n+1} = \sin(x_n)$$

(Hint: if  $\lim_n x_n = L$ , then what is  $\lim_n x_{n-1}$ ?)

3. Prove that, for  $b \in \mathbb{R}$  with  $b > 0$ ,  $x_n := \frac{n}{b^n}$  converges to 0 if  $b > 1$  and properly diverges to  $+\infty$  if  $b \leq 1$ .

4. Prove that

$$x_n := 1 + \frac{1}{2^2} + \cdots + \frac{1}{n^2} := \sum_{k=0}^n \frac{1}{k^2}$$

converges (don't try to find the limiting value).

5. Let  $x_1 \in \mathbb{R}$  be nonzero, and define inductively  $x_{n+1} := x_n + \frac{1}{x_n}$ . Prove that

$$\lim_{n \rightarrow \infty} x_n = \begin{cases} +\infty & x_1 > 0 \\ -\infty & x_1 < 0 \end{cases}.$$

## 1.2 (Functional Limits/Continuity)

1. ★ Let  $f : \mathbb{R} \rightarrow \mathbb{R}$  satisfy the following:

- i.  $f(x + y) = f(x) + f(y)$ , for all  $x, y \in \mathbb{R}$ ,
- ii.  $f$  continuous at 0
- iii.  $f(1) = 1$

Prove that  $f$  must be the identity function, i.e.  $f(x) = x$  for all  $x \in \mathbb{R}$ .

(Hint: begin by showing  $f$  must be continuous everywhere in  $\mathbb{R}$ , and use this to prove the claim for  $x \in \mathbb{Q}$ . Conclude by a density argument.)

2. [Recall that a set  $X \subset \mathbb{R}$  is said to be *open* if for every  $x \in X$ , there exists an  $\varepsilon > 0$  such that  $(x - \varepsilon, x + \varepsilon) \subset X$  (i.e., if a point is in  $X$ , so are all of its "neighboring" points for a sufficiently small neighborhood), and that a set  $Y \subset \mathbb{R}$  is said to be *closed* if its complement  $Y^C = \mathbb{R} \setminus Y$  is open.]

Let  $f : \mathbb{R} \rightarrow \mathbb{R}$  be continuous. Prove that  $X := \{x \in \mathbb{R} \mid f(x) = 0\}$  is a closed subset of  $\mathbb{R}$ .

(Bonus ★: what can you say about the set  $Y := \{x : a \leq f(x) < b\}$  for some real numbers  $a < b$ ? Can you find continuous functions  $f$  such that  $Y$  open, closed, both, and neither?)

3. Compute the following functional limits using only the  $\varepsilon$ - $\delta$ / $\varepsilon$ - $M$  definition:

$$a) \quad \lim_{x \rightarrow 1^+} \left( \frac{x}{x-1} \right)$$

$$b) \quad \lim_{x \rightarrow \infty} \left( \frac{\sqrt{x+1}}{x} \right)$$

$$c) \quad \lim_{x \rightarrow \infty} \frac{\sqrt{x} - x}{\sqrt{x} + x}$$

4. Let  $f : \mathbb{R}_+ \rightarrow \mathbb{R}$ , where  $\mathbb{R}_+ := \{x \in \mathbb{R} \mid x \geq 0\}$ . Prove that, for some real number  $L$ ,

$$\lim_{x \rightarrow \infty} f(x) = L \Leftrightarrow \lim_{x \rightarrow 0^+} f\left(\frac{1}{x}\right) = L.$$

5. We say a function  $f : \mathbb{R} \rightarrow \mathbb{R}$  is *Lipschitz continuous* if there exists a constant  $K > 0$  such that

$$|f(x) - f(y)| \leq K|x - y|, \quad \forall x, y \in \mathbb{R}.$$

Prove that if  $f$  Lipschitz continuous, it is also *uniformly* continuous. Can you find an example of a continuous function that isn't Lipschitz continuous?

(Bonus: prove that if  $f : [a, b] \rightarrow \mathbb{R}$  is differentiable with continuous derivative, then  $f$  is Lipschitz on  $[a, b]$ )

6. Prove using the  $\delta$ - $\varepsilon$  definition that the following functions are continuous on  $\mathbb{R}$ :

$$a) f(x) := \frac{1}{1+x^2}, \quad b) f(x) := \sqrt{x^2+1}.$$

7. ★ Let  $f : \mathbb{R}_+ \rightarrow \mathbb{R}$  be continuous and bounded. Show that for any  $T \in \mathbb{R}$ , there exists a sequence  $\{x_n\} \subset \mathbb{R}_+$  such that  $\lim_{n \rightarrow \infty} x_n = +\infty$  and

$$\lim_{n \rightarrow \infty} [f(x_n + T) - f(x_n)] = 0.$$

(Hint: this one's very hard)

8. Let  $f : [0, 1] \rightarrow \mathbb{R}$  be continuous, with  $f(0) = 0 = f(1)$ . Show that there must exist a  $c \in [0, \frac{1}{2}]$  such that  $f(c) = f(c + \frac{1}{2})$ .

(Hint: don't reinvent the wheel; turn what you have into a wheel)

9. Let  $f : [0, 1] \rightarrow \mathbb{R}$  continuous, and suppose that for every  $x \in [0, 1]$ , there exists a  $y \in [0, 1]$  such that

$$|f(y)| \leq \frac{1}{2}|f(x)|.$$

Prove that there exists a  $c \in [0, 1]$  such that  $f(c) = 0$ .

## 2 Solutions

### 2.1 Sequences

1. a) Remember that  $|\sin(x)| \leq 1$  for all  $x \in \mathbb{R}$ , thus

$$0 \leq \left| \frac{\sin(n)}{n} \right| \leq \frac{1}{n}.$$

Since  $\frac{1}{n}$  converges to zero, then by the squeeze theorem, so does  $\frac{\sin(n)}{n}$ .

- b) We can write

$$0 \leq \frac{n!}{n^n} = \frac{n \cdot (n-1) \cdots (1)}{\underbrace{n \cdots n}_{n \text{ times}}} = \underbrace{\frac{n}{n}}_{=1} \cdot \underbrace{\frac{n-1}{n}}_{\leq 1} \cdot \underbrace{\frac{n-2}{n}}_{\leq 1} \cdots \frac{1}{n} \leq \frac{1}{n},$$

so again  $\frac{n!}{n^n}$  converges to zero by squeeze theorem.

- c) Remember that  $1 + 2 + \cdots + n = \frac{(n)(n+1)}{2}$ , so that the sequence may be written

$$\begin{aligned} \frac{(1 + 2 + \cdots + n)^2}{n^4} &= \frac{((n)(n+1))^2}{4n^4} = \frac{n^2(n^2 + 2n + 1)}{4n^4} \\ &= \frac{n^4 + 2n^3 + n^2}{4n^4} = \frac{1}{4} + \frac{1}{2n} + \frac{1}{4n^2} \rightarrow \frac{1}{4}. \end{aligned}$$

2. a) We prove  $x_n$  is monotonically increasing and bounded from above, from which case convergence follows by the monotone convergence theorem. We prove both by induction. For increasing, the base case is clear, for  $x_2 = \sqrt{2 + \sqrt{2}} > \sqrt{2} = x_1$ . Supposing this inequality holds for some  $n$ , i.e.,  $x_n \geq x_{n-1}$ , we find that

$$x_{n+1} = \sqrt{2 + x_n} \stackrel{\text{induct}}{\geq} \sqrt{2 + x_{n-1}} \stackrel{\text{by def.}}{=} x_n,$$

so we have monotone increasing indeed. For boundedness, we claim  $x_n \leq 2$  for all  $n \geq 1$ . The base case, for  $n = 1$ , is clear. Supposing  $x_{n-1} \leq 2$ , then

$$x_n = \sqrt{2 + x_{n-1}} \stackrel{\text{induct}}{\leq} \sqrt{2 + 2} = 2,$$

so we indeed have boundedness of the whole sequence. Thus, we know  $x_n$  converges; let  $L$  be its limit. But then, we also know that  $x_n = \sqrt{2 + x_{n-1}}$ , thus

$$L = \lim_n x_n = \lim_n \sqrt{2 + x_{n-1}} \stackrel{\text{cnty of sqrt}}{=} \sqrt{2 + L}.$$

Squaring both sides, this means

$$L^2 = L + 2,$$

which one can solve to find two solutions,  $L = 2$  and  $L = -1$ . But  $x_n$  is a strictly positive, increasing sequence, so it can't have a negative limit, and thus we conclude  $L = 2$ .

- b) c) d)

- 3.
4. We will employ the Cauchy criterion to prove convergence. Let  $\varepsilon > 0$  and fix  $m > n \geq N$  for some  $N$  to be determined later. Then,

$$\begin{aligned}
|x_m - x_n| &= \left(1 + \frac{1}{2^2} + \dots + \frac{1}{m^2}\right) - \left(1 + \frac{1}{2^2} + \dots + \frac{1}{n^2}\right) \\
&= \frac{1}{(n+1)^2} + \frac{1}{(n+2)^2} + \dots + \frac{1}{m^2} \\
&\leq \frac{1}{(n+1)n} + \frac{1}{(n+1)(n+2)} + \dots + \frac{1}{m(m-1)} \\
&= \left(\frac{1}{n} - \frac{1}{n+1}\right) + \left(\frac{1}{n+1} - \frac{1}{n+2}\right) + \dots + \left(\frac{1}{m} - \frac{1}{m-1}\right) \\
&= \frac{1}{n} - \frac{1}{m} \leq \frac{1}{N},
\end{aligned}$$

so taking  $N \geq \frac{1}{\varepsilon}$  will work to prove convergence.

**Remark 2.1:** When I originally did this question, I immediately upper-bounded the second line by  $\frac{m-n}{(n+1)^2} \leq (m-n)\varepsilon$ , which is *not* good enough to prove the desired result.

5.

## 2.2 (Functional Limits/Continuity)

1. We follow the hint. First, we show  $f$  continuous everywhere. Before that, we note that  $f(0) = 0$ , for

$$f(0) = f(0+0) = f(0) + f(0) \Rightarrow f(0) = 0,$$

just by using the definition. Fix now  $\varepsilon > 0$ , and let  $\delta > 0$  such that  $|x| < \delta \Rightarrow |f(x) - f(0)| = |f(x)| < \varepsilon$ , appealing to the assumed continuity of  $f$  at 0. Then, for any  $x, y \in \mathbb{R}$  with  $|x - y| < \delta$ , we find

$$|f(x) - f(y)| \stackrel{\text{definition}}{=} |f(x - y)| < \varepsilon,$$

using the continuity assumption at the origin (*in particular, we have uniform convergence*).

Next, we prove the result for  $q \in \mathbb{Q}$ . First, remark that for any positive integer  $n$  and any  $x \in \mathbb{R}$ , we have that

$$f(nx) = f((n-1)x + x) = f((n-1)x) + f(x),$$

but we can repeat this work for  $f((n-1)x)$ , and we deduce that  $f(nx) = nf(x)$ . By similar reasoning, we can deduce that  $f(nx) = nf(x)$  for any negative integer as well. For  $q \in \mathbb{Q}$ , we can write

$$q = \frac{a}{b},$$

where  $a, b \in \mathbb{Z}$ . From the previous line of reasoning, we see thus that

$$f\left(\frac{a}{b}\right) = a \cdot f\left(\frac{1}{b}\right).$$

But also,

$$1 = f(1) = f\left(b \cdot \frac{1}{b}\right) = bf\left(\frac{1}{b}\right) \Rightarrow f\left(\frac{1}{b}\right) = \frac{1}{b},$$

from which we conclude

$$f(q) = f\left(\frac{a}{b}\right) = \frac{a}{b} = q$$

indeed. This proves the conclusion for all rational numbers. Now, for any  $x \in \mathbb{R}$ , let  $\{q_n\}$  be a sequence of rational numbers converging to  $x$ , which must exist by the density of  $\mathbb{Q}$  in  $\mathbb{R}$ . Then, by the continuity of  $f$  we proved above,

$$\lim_n f(q_n) = f(x)$$

on the one hand, but also, since  $q_n \in \mathbb{Q}$  for each  $n$ ,

$$\lim_n f(q_n) = \lim_n q_n = x,$$

from which we conclude  $f(x) = x$  for all  $x \in \mathbb{R}$ , as we aimed to show.

2. We will equivalently show that  $X^c = \{f(x) \neq 0\}$  is open. Let  $x \in X^c$ , and assume wlog that  $f(x) > 0$  (if  $f(x) < 0$ , repeat the proof with  $-f$  instead of  $f$ ), and let  $\varepsilon := \frac{f(x)}{2}$ , which is strictly positive since  $f(x) \neq 0$ . Since  $f$  continuous, in particular, at  $x$ , there exists a  $\delta > 0$  such that if  $|y - x| < \delta$ , then  $|f(y) - f(x)| < \varepsilon$ . But this means, for such  $y$ ,

$$\begin{aligned} |f(y) - f(x)| < \varepsilon &\Rightarrow \frac{-f(x)}{2} < f(y) - f(x) < \frac{f(x)}{2} \\ &\Rightarrow \frac{f(x)}{2} < f(y) < \frac{3f(x)}{2}, \end{aligned}$$

which, since  $f(x) > 0$ , in particular implies that if  $|y - x| < \delta$ , then  $f(y) > 0$ . This means that all such  $y \in X^c$  as well, i.e.  $(x - \delta, x + \delta) \subset X^c$ , which is exactly the definition of openness. Thus,  $X^c$  open and so  $X$  closed.

3.

- a) We claim the given limit diverges properly to  $+\infty$ . Let  $M > 0$ , and let  $\delta := \frac{1}{M} > 0$ . Then, if  $x$  is such that  $0 < x - 1 < \delta$ , then in particular  $x > 1$  and  $\frac{1}{x-1} > \frac{1}{\delta}$ , from which we conclude

$$\frac{x}{x-1} > \frac{1}{\delta} = M,$$

which proves the claim.

- b) We claim the given limit is 0. Fix  $\varepsilon > 0$ . Note that if the function in question was just  $\frac{\sqrt{x}}{x}$ , our job would be far easier, for this simplifies to  $\frac{1}{\sqrt{x}}$ , so just taking  $M := \frac{1}{\varepsilon^2}$  would do the trick. So, inspired by this work, we can rewrite the function in question:

$$f(x) := \frac{\sqrt{x+1}}{x} = \frac{\sqrt{x}}{x} \cdot \frac{\sqrt{x+1}}{\sqrt{x}} = \frac{1}{\sqrt{x}} \sqrt{1 + \frac{1}{x}}.$$

In particular, we've put all the  $x$  dependence into denominators, which should always be a goal when proving something goes to zero. Let now  $x > M$  with  $M := \frac{2}{\varepsilon^2}$ , assuming without loss of generality that  $\varepsilon < 1$ <sup>1</sup> then

---

<sup>1</sup>This is wlog since what really matters in limit proofs is small  $\varepsilon$ ; if you don't like this, you can instead take

$$M = \max\left(\frac{2}{\varepsilon^2}, 1\right),$$

$$f(x) < \frac{1}{\sqrt{M}} \sqrt{1 + \frac{1}{M}} = \frac{\varepsilon}{\sqrt{2}} \sqrt{1 + \varepsilon^2} < \frac{\varepsilon}{\sqrt{2}} \sqrt{2} = \varepsilon,$$

so the proof follows.

c) Whenever you see ugly functions like this, you should always simplify (in the sense of getting rid of as many  $x$ 's as possible) before attempting anything. We see that:

$$f(x) := \frac{\sqrt{x} - x}{\sqrt{x} + x} = \frac{-\sqrt{x} + x + 2\sqrt{x}}{\sqrt{x} + x} = -1 + 2 \frac{\sqrt{x}}{\sqrt{x} + x} = -1 + \frac{2}{1 + \sqrt{x}}.$$

In particular, we can see from here that  $\lim_{x \rightarrow \infty} f(x) = -1$ ; for  $\varepsilon > 0$  (and less than 1, wlog), let  $M := \left(\frac{2}{\varepsilon} - 1\right)^2$ , then for  $x > M$ ,

$$|f(x) - (-1)| = \frac{2}{1 + \sqrt{x}} < \frac{2}{1 + \sqrt{M}} = \varepsilon,$$

as we needed to show.

4. Assume the first direction. Let  $\varepsilon > 0$ . By definition, there exists  $M > 0$  such that  $x > M$  implies  $|f(x) - L| < \varepsilon$ . Taking  $\delta := \frac{1}{M}$ , then, this implies that for all  $y$  such that  $0 < \frac{1}{y} < \frac{1}{\delta}$ , (viewing  $x$  as  $\frac{1}{y}$ ) we have  $\left|f\left(\frac{1}{y}\right) - L\right| < \varepsilon$ , which  $\lim_{x \rightarrow 0^+} f\left(\frac{1}{x}\right) = L$ . The inverse implication is very similar.
5. Let  $\varepsilon > 0$  and let  $\delta := \frac{\varepsilon}{K}$ . Then,  $|x - y| < \delta$  implies  $|f(x) - f(y)| \leq K|x - y| < \frac{K}{K}\varepsilon = \varepsilon$ , so  $f$  continuous (uniformly). The classic example of a non-Lipschitz but continuous function is  $f(x) := x^2$  on  $\mathbb{R}$ ; to see this, it suffices to take  $y = 0$ . Then, we see that

$$|f(x) - f(y)| = x^2,$$

so any Lipschitz constant would have to be proportional to  $x$ , which contradicts the uniformity definition.

6.

- a) Fix  $\varepsilon > 0$ ,  $x \in \mathbb{R}$  and let  $y$  such that  $|x - y| < \delta$ , with  $\delta$  to be chosen. Note that this implies  $y \in (x - \delta, x + \delta)$ , so  $|y| \leq |x| + \delta$ . Then:

$$\begin{aligned} |f(x) - f(y)| &= \left| \frac{1}{1 + x^2} - \frac{1}{1 + y^2} \right| \\ &= \frac{|y^2 - x^2|}{(1 + x^2)(1 + y^2)} \\ &= \frac{|(y - x)(y + x)|}{(1 + x^2)(1 + y^2)} \\ &\leq |y - x||y + x| \\ &< \delta(|y| + |x|) < \delta(\delta + 2|x|). \end{aligned}$$

If  $x = 0$ , then we can just take  $\delta = \sqrt{\varepsilon}$ . Else,  $|x| > 0$ , so that with the choice

---

then in particular  $\frac{1}{M} < 1$  and  $\frac{1}{\sqrt{M}} < \frac{\varepsilon}{\sqrt{2}}$ , the the proof follows identically.

$$\delta := \delta(x, \varepsilon) = \min \left\{ 2|x|, \frac{\varepsilon}{4|x|} \right\} > 0,$$

we have that  $\delta < 2|x|$  and  $\delta < \frac{\varepsilon}{4|x|}$ , so that continuing our work above we get

$$|f(x) - f(y)| < \delta(\delta + 2|x|) < \frac{\varepsilon}{4|x|}(4|x|) = \varepsilon,$$

as needed.

b)

7. This is tricky. One way you can interpret the result is that, if  $f$  a continuous and bounded function, then it must be “eventually periodic” with arbitrary period  $T$ ; i.e., we can find some properly diverging sequence of  $\{x_n\}$  such that  $f(x_n + T) - f(x_n)$  converges to zero.

With this interpretation, we fix  $T \in \mathbb{R} \setminus \{0\}$  (if  $T = 0$  we’re done) and let  $g(x) := f(x + T) - f(x)$  for convenience. Consider the following three possibilities:

(i)  $f$  is identically zero outside of some bounded set, or  $f$  decays to zero as  $|x| \rightarrow \infty$ , i.e.  $\lim_{x \rightarrow +\infty} f(x) = 0$ ; in either case, we can take  $x_n := n$  and conclude (why?).

(ii)  $g$  changes sign infinitely often for sufficiently large  $x$ , i.e. for all  $n \in \mathbb{N}$ , there exists a  $y_n > n$  such that  $g(y_n) > 0 (< 0)$  iff  $g(n) < 0 (> 0)$ . In this case, we can construct an unbounded, increasing sequence  $\{y_n\} \subset \mathbb{R}$  such that  $\{g(y_n)\}$  alternates sign, i.e. if  $g(y_1) > 0$ , then  $g(y_2) < 0$ ,  $g(y_3) > 0$ , etc. Since  $f$  continuous, then by the intermediate value theorem, then we can find a sequence  $\{x_n\}$  such that:

- $x_n \in (y_n, y_{n+1})$  for each  $n \in \mathbb{N}$
- $g(x_n) = 0$  for all  $n \in \mathbb{N}$

Moreover, this first condition implies  $\lim_n x_n \geq \lim_n y_n = \infty$ , so  $\{x_n\}$  also diverges to infinity. The second condition moreover gives that  $f(x_n + T) - f(x_n) = 0$  identically, so the claim is proven.

(iii) Finally, if neither of the two previous conditions are satisfied, then we know  $g$  must eventually be strictly positive or negative, i.e. there must exist some sufficiently large  $M > 0$  such that  $x \geq M \Rightarrow g(x) > 0$  or  $g(x) < 0$  (indeed, if we couldn’t find such an  $M$ , two cases would be possible: either  $g$  identically zero beyond some sufficiently large value of  $x$ , in which case we enter case (i), or  $g$  alternates sign infinitely often for large  $x$ , in which case we are in case (ii)).

Suppose first  $g(x) > 0$  for  $x \geq M$ . This implies  $f(x + T) > f(x)$ ; if  $T > 0$ , we can inductively argue then that  $f(x + nT) > f(x)$  for all  $n \in \mathbb{N}$ . So, if we define the sequence  $x_n := M + (n - 1)T$ , we conclude that  $f(x_n) > f(x_{n-1})$  for all  $n \in \mathbb{N}$ . But then,  $\{f(x_n)\}$  a bounded (by assumption,  $f$  bounded) sequence which monotonically increases, so by the Monotone Convergence Theorem, we know  $\lim_n f(x_n)$  exists. In particular, this implies

$$\lim_n [f(x_n + T) - f(x_n)] = \lim_n f(x_{n+1}) - \lim_n f(x_n) = 0,$$

using our definition of  $x_n$ , which implies  $x_{n+1} = x_n + T$ ; so, we are done in this case. If on the other hand  $T < 0$ , then we similarly define  $x_n := M - (n - 1)T$ , and conclude similarly. Finally, if instead  $g(x) < 0$  for  $x \geq M$ , the same sequence gives rise to a monotonically decreasing sequence, and the conclusion is the same.

8. Let  $g(x) := f(x) - f\left(x + \frac{1}{2}\right)$  for  $x \in \left[0, \frac{1}{2}\right]$ . Then,  $g(0) = -f\left(\frac{1}{2}\right)$  and  $g\left(\frac{1}{2}\right) = f\left(\frac{1}{2}\right)$ ; in particular,  $g$  must change sign on the interval  $\left[0, \frac{1}{2}\right]$ , for  $g(0) = -g\left(\frac{1}{2}\right)$ . Thus, there must exist a  $c$  for which  $g(c) = 0$ , which, unravelling the definition of  $g$ , proves the assertion.
9. Let  $x_1 \in [0, 1]$  arbitrary. Let  $x_2 \in [0, 1]$  such that  $|f(x_2)| \leq \frac{1}{2}|f(x_1)|$ , which exists by hypothesis. Repeat this inductively, defining a sequence of  $\{x_n\} \subset [0, 1]$  such that  $|f(x_{n+1})| \leq \frac{1}{2}|f(x_n)|$  for each  $n \geq 1$ . In particular,  $\{x_n\}$  a bounded sequence of real numbers, and thus by the Bolzano-Weierstrauss Theorem, there exists a point  $c \in [0, 1]$  and a subsequence  $\{x_{n_k}\} \subset \{x_n\}$  such that  $x_{n_k}$  converges to  $c$ . By continuity,  $f(x_{n_k})$  converges to  $f(c)$ . In addition, we see that, applying the hypothesis inductively,

$$|f(x_n)| \leq \frac{1}{2}|f(x_{n-1})| \leq \left(\frac{1}{2}\right)^2 |f(x_{n-2})| \leq \dots \leq \left(\frac{1}{2}\right)^{n-1} |f(x_1)|.$$

Applying this bound to the subsequence, we conclude

$$|f(x_{n_k})| \leq \left(\frac{1}{2}\right)^{n_k-1} |f(x_1)|,$$

and, taking limits on both sides, we find

$$|f(c)| \leq |f(x_1)| \lim_k \left(\frac{1}{2}\right)^{n_k-1} = 0,$$

hence  $f(c) = 0$ , as we aimed to find.